\documentclass{article}
\usepackage{epsfig}
\pagestyle{empty}
\begin{document}
$a_i$
\pagebreak

$3k$
\pagebreak

$i$
\pagebreak

$a_{i,i} ... a_{i+k-1,i+k-1},$
\pagebreak

$a_{i+k,i} ... a_{i+3k-1,i+k-1}$
\pagebreak

$2^k$
\pagebreak

$i + 3k$
\pagebreak

$m$
\pagebreak

$j$
\pagebreak

$a_{j,i} ... a_{j,i+k-1}$
\pagebreak

$ i + k$
\pagebreak

$0 ... i-1$
\pagebreak

$i + 3k ... m$
\pagebreak

$k$
\pagebreak

$B_i$
\pagebreak

$x$
\pagebreak

$T_x$
\pagebreak

$a_{j,(i-1)k+1}, a_{j,(i-1)k+2} , ... , a_{j,(i-1)k+k}.$
\pagebreak

$a_{j,(i-1)k+1}, ... , a_{j,ik}$
\pagebreak

$h = 1,2, ... , c$
\pagebreak

$C_{jh} = C_{jh} + T_{xh}$
\pagebreak

$2^3$
\pagebreak

$2^l$
\pagebreak

$0.75 log_2(n)$
\pagebreak

$n$
\pagebreak

$min(a,b)$
\pagebreak

$b$
\pagebreak

$\mathbb{F}_2$
\pagebreak

\[ Y_m^m(x) = Y_0^0 \ \sqrt{ \prod_{k=1}^{m} \frac{2k+1}{2k} } \ \ (-1)^m \ (1-x^2)^{m/2} \]
\pagebreak

$ Y_0^0 = 1 $
\pagebreak

$ Y_0^0 = 1/\sqrt{4\pi} $
\pagebreak

$ (-1)^m $
\pagebreak

$ \sqrt{2m+1} $
\pagebreak

\[ a_l^m = \frac{2l-1}{\sqrt{(l+m)(l-m)}} \]
\pagebreak

\[ b_l^m = -\sqrt{\frac{(l-1+m)(l-1-m)}{(l+m)(l-m)}} \]
\pagebreak

\[ a_l^m = \sqrt{\frac{(2l+1)(2l-1)}{(l+m)(l-m)}} \]
\pagebreak

\[ b_l^m = -\sqrt{\frac{2l+1}{2l-3}\,\frac{(l-1+m)(l-1-m)}{(l+m)(l-m)}} \]
\pagebreak

$ P_0 = 1 $
\pagebreak

$ P_1 = x $
\pagebreak

\[ l P_l = (2l-1) x P_{l-1} - (l-1) P_{l-2} \]
\pagebreak

\end{document}
